theories/newth/SmtMap.ec
@@ -32,27 +32,31 @@ proof. by move=> m; apply/map_eqP=> x; rewrite offunE. qed.
 
 (* -------------------------------------------------------------------- *)
 lemma nosmt setE ['a 'b] (m : ('a, 'b) map) x v : 
-  m.[x <- v] = offun (fun y => if x = y then v else m.[y]).
+  m.[x <- v] = offun (fun y => if y = x then v else m.[y]).
 proof. by apply/map_eqP=> y /=; rewrite offunE /#. qed.
 
+(* -------------------------------------------------------------------- *)
 lemma nosmt getE ['a 'b] (m : ('a, 'b) map) x : m.[x] = (tofun m) x.
 proof. by []. qed.
 
 (* -------------------------------------------------------------------- *)
 lemma nosmt get_setE ['a 'b] (m : ('a, 'b) map) (x y : 'a) b :
-  m.[x <- b].[y] = if x = y then b else m.[y].
+  m.[x <- b].[y] = if y = x then b else m.[y].
 proof. by rewrite setE getE offunK. qed.
 
+(* -------------------------------------------------------------------- *)
 lemma nosmt get_set_sameE (m : ('a,'b) map) (x : 'a) b :
   m.[x <- b].[x] = b.
 proof. by rewrite get_setE. qed.
 
+(* -------------------------------------------------------------------- *)
 lemma nosmt get_set_eqE (m : ('a, 'b) map) (x y : 'a) b :
-  x = y => m.[x <- b].[y] = b.
+  y = x => m.[x <- b].[y] = b.
 proof. by move=> <-; rewrite get_set_sameE. qed.
 
+(* -------------------------------------------------------------------- *)
 lemma nosmt get_set_neqE (m : ('a, 'b) map) (x y : 'a) b :
-  x <> y => m.[x <- b].[y] = m.[y].
+  y <> x => m.[x <- b].[y] = m.[y].
 proof. by rewrite get_setE => ->. qed.
 
 (* -------------------------------------------------------------------- *)
@@ -63,28 +67,33 @@ proof. by smt(). qed.
 op map ['a 'b 'c] (f : 'a -> 'b -> 'c) (m : ('a, 'b) map) = 
    offun (fun x => f x m.[x]).
 
+(* -------------------------------------------------------------------- *)
 lemma mapE ['a 'b 'c] (f : 'a -> 'b -> 'c) (m : ('a, 'b) map) x :
   (map f m).[x] = f x m.[x].
 proof. by rewrite /map getE offunK. qed.
 
+(* -------------------------------------------------------------------- *)
 lemma map_set (f : 'a -> 'b -> 'c) (m : ('a, 'b) map) x b :
   map f (m.[x <- b]) = (map f m).[x <- f x b].
 proof.
 apply/map_eqP => y; rewrite mapE !get_setE.
-by case: (x = y) => //; rewrite mapE.
+by case: (y = x) => //; rewrite mapE.
 qed.
 
 (* -------------------------------------------------------------------- *)
 op eq_except ['a 'b] X (m1 m2 : ('a, 'b) map) =
   forall y, !X y => m1.[y] = m2.[y].
 
+(* -------------------------------------------------------------------- *)
 lemma nosmt eq_except_refl ['a 'b] X : reflexive (eq_except<:'a, 'b> X).
 proof. by []. qed.
 
+(* -------------------------------------------------------------------- *)
 lemma nosmt eq_except_sym ['a 'b] X (m1 m2 : ('a, 'b) map) :
   eq_except X m1 m2 => eq_except X m2 m1.
 proof. by move=> h x /h ->. qed.
 
+(* -------------------------------------------------------------------- *)
 lemma nosmt eq_except_trans ['a 'b] X (m2 m1 m3 : ('a, 'b) map) :
   eq_except X m1 m2 => eq_except X m2 m3 => eq_except X m1 m3.
 proof. by move=> h1 h2 x ^/h1 -> /h2 ->. qed.
@@ -129,17 +138,25 @@ axiom ofmapK ['a 'b] (m : ('a, 'b option) map) :
 axiom isfmap_offmap (m : ('a, 'b) fmap) :
   is_finite (fun x => (tomap m).[x] <> None).
 
-lemma nosmt finite_dom (m : ('a, 'b) fmap) :
+(* -------------------------------------------------------------------- *)
+lemma nosmt finite_dom ['a 'b] (m : ('a, 'b) fmap) :
   is_finite (dom m).
 proof. exact/isfmap_offmap. qed.
 
-lemma nosmt finite_rng (m : ('a, 'b) fmap) :
-  is_finite (rng m).
+(* -------------------------------------------------------------------- *)
+lemma nosmt finite_rng ['a 'b] (m : ('a, 'b) fmap) : is_finite (rng m).
 proof.
-exists (undup (map (fun x=> oget m.[x]) (to_seq (dom m)))); split.
-+ exact/undup_uniq.
-move=> y; rewrite rngE mem_undup mapP /=; apply/exists_iff=> /= x.
-by rewrite mem_to_seq 1:finite_dom domE; case: (m.[x]).
+pose s := map (fun x => oget m.[x]) (to_seq (dom m)).
+apply/finiteP; exists s => y; rewrite rngE /= => -[x mxE].
+by apply/mapP; exists x => /=; rewrite mem_to_seq 1:finite_dom domE mxE.
+qed.
+
+(* -------------------------------------------------------------------- *)
+lemma nosmt fmap_eqP ['a 'b] (m1 m2 : ('a, 'b) fmap) :
+  (forall x, m1.[x] = m2.[x]) <=> m1 = m2.
+proof.
+split=> [pw_eq|->] //; rewrite -tomapK -(tomapK m2).
+by congr; apply/Map.map_eqP=> x; rewrite pw_eq.
 qed.
 
 (* -------------------------------------------------------------------- *)
@@ -150,39 +167,72 @@ proof.
 by rewrite /empty ofmapK //; exists [] => /= x; rewrite Map.cstE.
 qed.
 
+(* -------------------------------------------------------------------- *)
 lemma emptyE ['a 'b] x : empty<:'a, 'b>.[x] = None.
 proof. by rewrite getE empty_valE Map.cstE. qed.
 
+(* -------------------------------------------------------------------- *)
 lemma mem_empty ['a 'b] x : x \notin empty<:'a, 'b>.
 proof. by rewrite domE emptyE. qed.
+
+(* -------------------------------------------------------------------- *)
+lemma mem_rng_empty ['a 'b] y : !rng empty<:'a, 'b> y.
+proof. by rewrite rngE /= negb_exists=> /= x; rewrite emptyE. qed.
 
 (* -------------------------------------------------------------------- *)
 lemma nosmt set_valE ['a 'b] (m : ('a, 'b) fmap) x v :
   tomap m.[x <- v] = (tomap m).[x <- Some v].
 proof.
 pose s := to_seq (fun x => (tomap m).[x] <> None).
-rewrite /"_.[_<-_]" ofmapK //; exists (undup (x :: s)).
-split; [by rewrite undup_uniq | move=> y; rewrite mem_undup].
-case: (y = x) => [|^neq] ->/=; first by rewrite Map.get_set_sameE.
-by rewrite Map.get_set_neqE 1:eq_sym //; apply/mem_to_seq/isfmap_offmap.
+rewrite /"_.[_<-_]" ofmapK //; apply/finiteP; exists (x :: s).
+move=> y /=; rewrite Map.get_setE; case: (y = x) => //=.
+by move=> ne_yx h; apply/mem_to_seq/h/isfmap_offmap.
 qed.
 
 (* --------------------------------------------------------------------- *)
 lemma get_setE ['a 'b] (m : ('a, 'b) fmap) (x y : 'a) b :
-  m.[x <- b].[y] = if x = y then Some b else m.[y].
+  m.[x <- b].[y] = if y = x then Some b else m.[y].
 proof. by rewrite /"_.[_]" /"_.[_<-_]" set_valE Map.get_setE. qed.
 
+(* -------------------------------------------------------------------- *)
 lemma nosmt get_set_sameE (m : ('a,'b) fmap) (x : 'a) b :
   m.[x <- b].[x] = Some b.
 proof. by rewrite get_setE. qed.
 
+(* -------------------------------------------------------------------- *)
 lemma nosmt get_set_eqE (m : ('a, 'b) fmap) (x y : 'a) b :
-  x = y => m.[x <- b].[y] = Some b.
+  y = x => m.[x <- b].[y] = Some b.
 proof. by move=> <-; rewrite get_set_sameE. qed.
 
+(* -------------------------------------------------------------------- *)
 lemma nosmt get_set_neqE (m : ('a, 'b) fmap) (x y : 'a) b :
-  x <> y => m.[x <- b].[y] = m.[y].
+  y <> x => m.[x <- b].[y] = m.[y].
 proof. by rewrite get_setE => ->. qed.
+
+(* -------------------------------------------------------------------- *)
+lemma nosmt set_setE (m : ('a, 'b) fmap) x x' b b' :
+  m.[x <- b].[x' <- b']
+    = (x' = x) ? m.[x' <- b'] : m.[x' <- b'].[x <- b].
+proof.
+apply/fmap_eqP=> y; rewrite !get_setE; case: (x' = x)=> //= [<<-|].
++ by rewrite !get_setE; case: (y = x').
++ by rewrite !get_setE; case: (y = x')=> //= ->> ->.
+qed.
+
+(* -------------------------------------------------------------------- *)
+lemma nosmt set_set_sameE (m : ('a, 'b) fmap) (x : 'a) b b' :
+  m.[x <- b].[x <- b'] = m.[x <- b'].
+proof. by rewrite set_setE. qed.
+
+(* -------------------------------------------------------------------- *)
+lemma nosmt set_set_eqE (m : ('a, 'b) fmap) (x x' : 'a) b b' :
+  x' = x => m.[x <- b].[x' <- b'] = m.[x <- b'].
+proof. by rewrite set_setE. qed.
+
+(* -------------------------------------------------------------------- *)
+lemma nosmt set_set_neqE (m : ('a, 'b) fmap) (x x' : 'a) b b' :
+  x' <> x => m.[x <- b].[x' <- b'] = m.[x' <- b'].[x <- b].
+proof. by rewrite set_setE => ->. qed.
 
 (* -------------------------------------------------------------------- *)
 op rem ['a 'b] (m : ('a, 'b) fmap) x =
@@ -194,42 +244,177 @@ lemma nosmt rem_valE ['a 'b] (m : ('a, 'b) fmap) x :
 proof.
 rewrite /rem ofmapK //; pose P z := (tomap m).[z] <> None.
 apply/(finite_leq P)/isfmap_offmap => y @/P.
-by rewrite !Map.get_setE; case: (x = y).
+by rewrite !Map.get_setE; case: (y = x).
 qed.
 
 (* -------------------------------------------------------------------- *)
-lemma nosmt remE ['a 'b] (m : ('a, 'b) fmap) x y :
-  (rem m x).[y] = if x = y then None else m.[y].
+lemma remE ['a 'b] (m : ('a, 'b) fmap) x y :
+  (rem m x).[y] = if y = x then None else m.[y].
 proof. by rewrite /rem /"_.[_]" rem_valE Map.get_setE. qed.
 
 (* -------------------------------------------------------------------- *)
 lemma mem_set ['a 'b] (m : ('a, 'b) fmap) x b y :
   y \in m.[x <- b] <=> (y \in m \/ y = x).
-proof. by rewrite !domE get_setE (eq_sym x y); case: (y = x). qed.
+proof. by rewrite !domE get_setE; case: (y = x). qed.
 
 (* -------------------------------------------------------------------- *)
 lemma mem_rem ['a 'b] (m : ('a, 'b) fmap) x y :
   y \in (rem m x) <=> (y \in m /\ y <> x).
-proof. by rewrite !domE remE (eq_sym x y); case: (y = x) => //=. qed.
+proof. by rewrite !domE remE; case: (y = x) => //=. qed.
 
 (* -------------------------------------------------------------------- *)
 op eq_except ['a 'b] X (m1 m2 : ('a, 'b) fmap) =
   Map.eq_except X (tomap m1) (tomap m2).
 
+(* -------------------------------------------------------------------- *)
 lemma eq_except_refl ['a 'b] X : reflexive (eq_except<:'a, 'b> X).
 proof. by apply/Map.eq_except_refl<:'a, 'b option>. qed.
 
+(* -------------------------------------------------------------------- *)
 lemma eq_except_sym ['a 'b] X (m1 m2 : ('a, 'b) fmap) :
   eq_except X m1 m2 => eq_except X m2 m1.
 proof. by apply/Map.eq_except_sym<:'a, 'b option>. qed.
 
+(* -------------------------------------------------------------------- *)
 lemma eq_except_trans ['a 'b] X (m1 m2 m3 : ('a, 'b) fmap) :
   eq_except X m1 m2 => eq_except X m2 m3 => eq_except X m1 m3.
 proof. by apply/Map.eq_except_trans<:'a, 'b option>. qed.
 
+(* -------------------------------------------------------------------- *)
 lemma eq_exceptP ['a 'b] X (m1 m2 : ('a, 'b) fmap) :
   eq_except X m1 m2 <=> (forall x, !X x => m1.[x] = m2.[x]).
 proof. by split=> h x /h. qed.
+
+(* -------------------------------------------------------------------- *)
+lemma eq_except0 ['a 'b] (m1 m2 : ('a, 'b) fmap) :
+  eq_except pred0 m1 m2 <=> m1 = m2.
+proof. by rewrite eq_exceptP /pred0 /= fmap_eqP. qed.
+
+(* -------------------------------------------------------------------- *)
+lemma eq_exceptSm ['a 'b] X x y (m1 m2 : ('a, 'b) fmap) :
+     eq_except X m1 m2
+  => eq_except (predU X (pred1 x)) m1.[x <- y] m2.
+proof.
+move=> eqeX_m1_m2; rewrite eq_exceptP=> x0; rewrite get_setE /predU /pred1.
+by move=> /negb_or []; move: eqeX_m1_m2=> /eq_exceptP h /h -> ->.
+qed.
+
+(* -------------------------------------------------------------------- *)
+lemma eq_exceptmS ['a 'b] X x y (m1 m2 : ('a, 'b) fmap) :
+     eq_except X m1 m2
+  => eq_except (predU X (pred1 x)) m1 m2.[x <- y].
+proof. by move=> h; apply/eq_except_sym/eq_exceptSm/eq_except_sym. qed.
+
+(* -------------------------------------------------------------------- *)
+lemma eq_except_setl ['a 'b] x y (m : ('a, 'b) fmap) :
+  eq_except (pred1 x) m.[x <- y] m.
+proof.
+have ->: pred1 x = predU pred0 (pred1 x) by exact/fun_ext.
+by apply/eq_exceptSm/eq_except0.
+qed.
+
+(* -------------------------------------------------------------------- *)
+lemma eq_except_setr ['a 'b] x y (m : ('a, 'b) fmap) :
+  eq_except (pred1 x) m m.[x <- y].
+proof. by apply/eq_except_sym/eq_except_setl. qed.
+
+(* -------------------------------------------------------------------- *)
+lemma eq_except_set ['a 'b] X x y y' (m1 m2 : ('a, 'b) fmap) :
+  eq_except X m1 m2 =>
+  eq_except ((y <> y') ? predU X (pred1 x) : X) m1.[x <- y] m2.[x <- y'].
+proof.
+move=> /eq_exceptP h; case: (y = y') => /= [<-|].
+  by apply/eq_exceptP=> z _; rewrite !get_setE h.
+move=> ne_y_y'; apply/eq_exceptP=> z; rewrite negb_or.
+by case=> /h; rewrite !get_setE => + @/pred1 -> - ->.
+qed.
+
+(* -------------------------------------------------------------------- *)
+lemma nosmt eq_except_set_eq ['a 'b] X x y (m1 m2 : ('a, 'b) fmap) :
+  eq_except X m1 m2 => eq_except X m1.[x <- y] m2.[x <- y].
+proof. by move=> /(@eq_except_set _ x y y). qed.
+
+(* -------------------------------------------------------------------- *)
+lemma nosmt eq_except_set_same ['a 'b] X x y y' (m1 m2 : ('a, 'b) fmap) :
+     y = y'
+  => eq_except X m1 m2
+  => eq_except X m1.[x <- y] m2.[x <- y'].
+proof. by move=> <-; apply/eq_except_set_eq. qed.
+
+(* -------------------------------------------------------------------- *)
+lemma nosmt eq_except_set_neq ['a 'b] X x y y' (m1 m2 : ('a, 'b) fmap) :
+     y <> y'
+  => eq_except X m1 m2
+  => eq_except (predU X (pred1 x)) m1.[x <- y] m2.[x <- y'].
+proof. by move=> + /(@eq_except_set _ x y y' _ _)=> ->. qed.
+
+(* -------------------------------------------------------------------- *)
+op map ['a 'b 'c] (f : 'a -> 'b -> 'c) (m : ('a, 'b) fmap) = 
+  ofmap (Map.map (fun x => omap (f x)) (tomap m)).
+
+(* -------------------------------------------------------------------- *)
+lemma map_valE ['a 'b 'c] (f : 'a -> 'b -> 'c) m :
+  tomap (map f m) = Map.map (fun k => omap (f k)) (tomap m).
+proof.
+rewrite /map ofmapK //; pose P z := (tomap m).[z] <> None.
+apply/(finite_leq P)/isfmap_offmap => y @/P.
+by rewrite Map.getE Map.offunK /=; case: (tomap m).[y].
+qed.
+
+(* -------------------------------------------------------------------- *)
+lemma mapE ['a 'b 'c] (f : 'a -> 'b -> 'c) m x :
+  (map f m).[x] = omap (f x) m.[x].
+proof. by rewrite /map /"_.[_]" map_valE Map.mapE. qed.
+
+(* -------------------------------------------------------------------- *)
+lemma mem_map ['a 'b 'c] (f : 'a -> 'b -> 'c) m x :
+  x \in map f m <=> x \in m.
+proof. by rewrite !domE mapE iff_negb; case: (m.[x]). qed.
+
+(* -------------------------------------------------------------------- *)
+lemma map_set (f : 'a -> 'b -> 'c) m x b :
+  map f (m.[x <- b]) = (map f m).[x <- f x b].
+proof.
+apply/fmap_eqP => y; rewrite mapE !get_setE.
+by case: (y = x) => //; rewrite mapE.
+qed.
+
+(* -------------------------------------------------------------------- *)
+lemma map_comp ['a 'b 'c 'd]
+  (f : 'a -> 'b -> 'c) (g : 'a -> 'c -> 'd) m
+: map g (map f m) = map (fun a b => g a (f a b)) m.
+proof. by apply/fmap_eqP => a; rewrite !mapE; case: (m.[a]). qed.
+
+(* -------------------------------------------------------------------- *)
+op filter ['a 'b] (p : 'a -> 'b -> bool) m =
+  ofmap (Map.offun (fun x => oapp (p x) false m.[x] ? m.[x] : None)).
+
+(* -------------------------------------------------------------------- *)
+lemma filter_valE ['a 'b] (p : 'a -> 'b -> bool) m :
+  tomap (filter p m) =
+    Map.offun (fun x => oapp (p x) false m.[x] ? m.[x] : None).
+proof.
+rewrite /filter ofmapK //; pose P z := (tomap m).[z] <> None.
+apply/(finite_leq P)/isfmap_offmap => y @/P.
+by rewrite !Map.getE Map.offunK /= getE; case: (tomap m).[y].
+qed.
+
+(* -------------------------------------------------------------------- *)
+lemma filterE ['a 'b] (p : 'a -> 'b -> bool) m x :
+  (filter p m).[x] = oapp (p x) false m.[x] ? m.[x] : None.
+proof. by rewrite /filter /"_.[_]" filter_valE Map.offunE. qed.
+
+(* -------------------------------------------------------------------- *)
+lemma filter_set (p : 'a -> 'b -> bool) m x b :
+  filter p (m.[x <- b]) = p x b ? (filter p m).[x <- b] : rem (filter p m) x.
+proof.
+apply/fmap_eqP => y; rewrite !filterE !get_setE.
+case: (y = x) => [->|] /=; case: (p x b) => /=.
++ by rewrite get_setE.
++ by rewrite remE.
++ by rewrite get_setE=> + -> /=; rewrite filterE.
++ by rewrite remE=> + -> /=; rewrite filterE.
+qed.
 
 (* ==================================================================== *)
 op fdom ['a 'b] (m : ('a, 'b) fmap) =
@@ -237,18 +422,28 @@ op fdom ['a 'b] (m : ('a, 'b) fmap) =
 
 lemma mem_fdom ['a 'b] (m : ('a, 'b) fmap) (x : 'a) :
   x \in fdom m <=> x \in m.
-proof. by rewrite fdomE mem_oflist mem_to_seq ?isfmap_offmap. qed.
+proof. by rewrite fdomE mem_oflist mem_to_seq ?isfmap_offmap. qed.  
 
 (* -------------------------------------------------------------------- *)
 lemma fdom0 ['a 'b] : fdom empty<:'a, 'b> = fset0.
 proof. by apply/fsetP=> x; rewrite mem_fdom mem_empty in_fset0. qed.
 
-lemma nosmt fdom_set ['a 'b] (m : ('a, 'b) fmap) x v :
+(* -------------------------------------------------------------------- *)
+lemma fdom_eq0 ['a 'b] (m : ('a, 'b) fmap) : fdom m = fset0 => m = empty.
+proof.
+rewrite fsetP -fmap_eqP=> h x; rewrite emptyE.
+have ->: m.[x] = None <=> x \notin m by done.
+by rewrite -mem_fdom h in_fset0.
+qed.
+
+(* -------------------------------------------------------------------- *)
+lemma fdom_set ['a 'b] (m : ('a, 'b) fmap) x v :
   fdom m.[x <- v] = fdom m `|` fset1 x.
 proof.
 by apply/fsetP=> y; rewrite in_fsetU1 !mem_fdom mem_set.
 qed.
 
+(* -------------------------------------------------------------------- *)
 lemma fdom_rem ['a 'b] (m : ('a, 'b) fmap) x :
   fdom (rem m x) = fdom m `\` fset1 x.
 proof. 
@@ -265,35 +460,13 @@ lemma mem_fdom_rem ['a 'b] (m : ('a, 'b) fmap) x y :
 proof. by rewrite fdom_rem in_fsetD1. qed.
 
 (* ==================================================================== *)
-op card ['a 'b] (m : ('a, 'b) fmap) =
-  size (to_seq (dom m)) axiomatized by cardE.
+op frng ['a 'b] (m : ('a, 'b) fmap) =
+  oflist (to_seq (rng m)) axiomatized by frngE.
+
+lemma mem_frng ['a 'b] (m : ('a, 'b) fmap) (y : 'b) :
+  y \in frng m <=> rng m y.
+proof. by rewrite frngE mem_oflist mem_to_seq ?finite_rng. qed.  
 
 (* -------------------------------------------------------------------- *)
-lemma nosmt fdom_card ['a 'b] (m : ('a, 'b) fmap) :
-  card (fdom m) = card m.
-proof.
-rewrite fdomE cardE FSet.cardE -(perm_eq_size _ _ (oflistK _)).
-by rewrite undup_id // uniq_to_seq ?isfmap_offmap.
-qed.
-
-(* -------------------------------------------------------------------- *)
-lemma card0 ['a 'b] : card<:'a, 'b> empty = 0.
-proof. by rewrite -fdom_card fdom0 fcards0. qed.
-
-lemma card_set ['a 'b] (m : ('a, 'b) fmap) x v :
-  card m.[x <- v] = card m + b2i (x \notin m).
-proof.
-rewrite -fdom_card fdom_set; case: (x \in m) => /= h.
-+ rewrite fsetUC subset_fsetU_id -?fdom_card //.
-  by move=> y /in_fset1 ->; rewrite mem_fdom.
-+ rewrite fcardUI_indep ?fcard1 -?fdom_card //.
-  apply/fsetP=> y; rewrite in_fsetI mem_fdom.
-  by rewrite in_fset1 in_fset0; case: (y = x).
-qed.
-
-lemma card_rem ['a 'b] (m : ('a, 'b) fmap) x :
-  card (rem m x) = card m - b2i (x \in m).
-proof.
-rewrite -!fdom_card fdom_rem (fcardD1 (fdom m) x).
-by rewrite /b2i mem_fdom -addzA; case: (x \in m).
-qed.
+lemma frng0 ['a 'b] : frng empty<:'a, 'b> = fset0.
+proof. by apply/fsetP=> x; rewrite mem_frng mem_rng_empty in_fset0. qed.
